MemDevice.v
@@ -1,0 +1,61 @@
+Require Import Kami.All.
+Require Import FU.
+Require Import PMemDevice.
+Require Import MMappedRegs.
+
+Section mem_devices.
+  Variable name: string.
+  Variable Xlen_over_8: nat.
+  Variable Rlen_over_8: nat.
+  Variable mem_params : MemParamsType.
+  Variable ty: Kind -> Type.
+
+  Local Notation Xlen := (Xlen_over_8 * 8).
+  Local Notation PAddrSz := (Xlen).
+  Local Notation MemDevice := (@MemDevice Rlen_over_8 PAddrSz ty).
+  Local Notation mMappedRegDevice := (@mMappedRegDevice name Xlen_over_8 Rlen_over_8 ty).
+  Local Notation pMemDevice := (@pMemDevice name Xlen_over_8 Rlen_over_8 mem_params ty).
+
+  Open Scope kami_expr.
+  Open Scope kami_action.
+
+  Definition mem_devices
+    :  list MemDevice
+    := [
+         mMappedRegDevice;
+         pMemDevice
+       ].
+
+  Definition DeviceTag := Bit (Nat.log2_up (length mem_devices)).
+
+  (*
+    Note: we assume that device tags will always be valid given
+    the constraints we apply in generating them.
+  *)
+  Definition mem_device_apply
+    (k : Kind)
+    (tag : DeviceTag @# ty)
+    (f : MemDevice -> ActionT ty k)
+    :  ActionT ty k
+    := LETA result
+         :  Maybe k
+         <- snd
+              (fold_left
+                (fun acc device
+                  => (S (fst acc),
+                      LETA acc_result : Maybe k <- snd acc;
+                      If #acc_result @% "valid" || $(fst acc) != tag
+                        then Ret #acc_result
+                        else
+                          LETA result : k <- f device;
+                          Ret (Valid #result : Maybe k @# ty)
+                        as result;
+                      Ret #result))
+                mem_devices
+                (0, Ret Invalid));
+      Ret (#result @% "data").
+
+  Close Scope kami_action.
+  Close Scope kami_expr.
+
+End mem_devices.
