MemTable.v
@@ -1,0 +1,61 @@
+(*
+  physical device (pMemDevice) -> memory devices (MemDevices) -> memory table (MemTableEntry) -> physicalMem.v (MemRegion)
+*)
+Require Import Kami.All.
+Require Import FU.
+Require Import MemDevice.
+Require Import BinNums.
+Import BinNat.
+
+Section mem_table.
+  Variable name: string.
+  Variable Xlen_over_8: nat.
+  Variable Rlen_over_8: nat.
+  Variable mem_params : MemParamsType.
+  Variable ty: Kind -> Type.
+
+  Local Notation lgMemSz := (mem_params_size mem_params).
+  Local Notation mem_devices := (@mem_devices name Xlen_over_8 Rlen_over_8 mem_params ty).
+
+  Record MemTableEntry
+    := {
+         mtbl_entry_addr : N;
+         mtbl_entry_width : N;
+         mtbl_entry_device : option (Fin.t (length mem_devices))
+       }.
+
+  Ltac nat_deviceTag n
+    := exact
+         (@of_nat_lt n (length mem_devices)
+           (ltac:(repeat (try (apply le_n); apply le_S)))).
+
+  Local Definition mem_table
+    := [
+         {|
+           mtbl_entry_addr := 0%N;
+           mtbl_entry_width := 16%N;
+           mtbl_entry_device := Some ltac:(nat_deviceTag 0)
+         |};
+         {|
+           mtbl_entry_addr := N.pow 2 31; (* 80000000 *)
+           mtbl_entry_width := N.pow 2 (N.of_nat lgMemSz);
+           mtbl_entry_device := Some ltac:(nat_deviceTag 1)
+         |}
+       ].
+
+  Local Fixpoint sort_insert (A : Type) (f : A -> N) (x : A) (ys : list A)
+    :  list A
+    := match ys with
+         | [] => [x]
+         | y0 :: ys
+           => if N.leb (f x) (f y0)
+                then x :: y0 :: ys
+                else y0 :: (sort_insert f x ys)
+         end.
+
+  Local Definition sort : list MemTableEntry -> list MemTableEntry
+    := fold_right (sort_insert mtbl_entry_addr) [].
+
+  Definition sorted_mem_table := sort mem_table.
+
+End mem_table.
