PMemDevice.v
@@ -1,0 +1,73 @@
+Require Import Kami.All.
+Require Import FU.
+
+Section mem_devices.
+  Variable name: string.
+  Variable Xlen_over_8: nat.
+  Variable Rlen_over_8: nat.
+  Variable mem_params : MemParamsType.
+  Variable ty: Kind -> Type.
+
+  Local Notation "^ x" := (name ++ "_" ++ x)%string (at level 0).
+  Local Notation Rlen := (Rlen_over_8 * 8).
+  Local Notation Xlen := (Xlen_over_8 * 8).
+  Local Notation Data := (Bit Rlen).
+  Local Notation PAddrSz := (Xlen).
+  Local Notation PAddr := (Bit PAddrSz).
+  Local Notation MemWrite := (MemWrite Rlen_over_8 PAddrSz).
+  Local Notation lgMemSz := (mem_params_size mem_params).
+  Local Notation MemDevice := (@MemDevice Rlen_over_8 PAddrSz ty).
+
+  Open Scope kami_expr.
+  Open Scope kami_action.
+
+  Local Definition pMemRead (index: nat) (mode : PrivMode @# ty) (addr: PAddr @# ty)
+    : ActionT ty Data
+    := Call result
+         : Array Rlen_over_8 (Bit 8)
+         <- (^"readMem" ++ (natToHexStr index)) (SignExtendTruncLsb _ addr: Bit lgMemSz);
+       System [
+         DispString _ ("[pMemRead] index: " ++ natToHexStr index ++ "\n");
+         DispString _ "[pMemRead] addr: ";
+         DispHex addr;
+         DispString _ "\n";
+         DispString _ "[pMemRead] result: ";
+         DispHex #result;
+         DispString _ "\n"
+       ];
+       Ret (pack #result).
+
+  Local Definition pMemWrite (mode : PrivMode @# ty) (pkt : MemWrite @# ty)
+    : ActionT ty Void
+    := LET writeRq
+         :  WriteRqMask lgMemSz Rlen_over_8 (Bit 8)
+         <- (STRUCT {
+               "addr" ::= SignExtendTruncLsb lgMemSz (pkt @% "addr");
+               "data" ::= unpack (Array Rlen_over_8 (Bit 8)) (pkt @% "data");
+               "mask" ::= pkt @% "mask"
+             } : WriteRqMask lgMemSz Rlen_over_8 (Bit 8) @# ty);
+       Call ^"writeMem"(#writeRq: _);
+       System [
+         DispString _ "[pMemWrite] pkt: ";
+         DispHex pkt;
+         DispString _ "\n";
+         DispString _ "[pMemWrite] writeRq: ";
+         DispHex #writeRq;
+         DispString _ "\n"
+       ];
+       Retv.
+
+  Definition pMemDevice
+    :  MemDevice
+    := {|
+         mem_device_read := pMemRead;
+         mem_device_write
+           := fun (mode : PrivMode @# ty) (pkt : MemWrite @# ty)
+                => LETA _ <- pMemWrite mode pkt;
+                   Ret $$false
+       |}.
+
+  Close Scope kami_action.
+  Close Scope kami_expr.
+
+End mem_devices.
